more faithful to Mazza, with explicit applicative depth

thys/Untyped_Lambda_Calculus/ILC_UBeta_depth.thy
@@ -1,53 +1,8 @@
 (* version of uniform (parallel) reduction that tracks the applicative depth 
 (i.e., the number of application operators on top of) of the affected redex (\<Rightarrow>d from Mazza) *)
 theory ILC_UBeta_depth
-imports ILC_uniform
+imports ILC_Head_Reduction
 begin
-
-(* head reduction: *)
-definition hred :: "ivar iterm \<Rightarrow> ivar iterm \<Rightarrow> bool" where 
-"hred e e' \<equiv> \<exists> xs e1 es2. e = iApp (iLam xs e1) es2 \<and> e' = itvsubst (imkSubst xs es2) e1"
-
-lemma hred_irrename: "bij \<sigma> \<Longrightarrow> |supp \<sigma>| <o |UNIV::ivar set| \<Longrightarrow> hred e e' \<Longrightarrow> hred (irrename \<sigma> e) (irrename \<sigma> e')"
-unfolding hred_def apply(elim exE) subgoal for xs e1 es2
-  apply(rule exI[of _ "dsmap \<sigma> xs"])
-  apply(rule exI[of _ "irrename \<sigma> e1"])  
-  apply(rule exI[of _ "smap (irrename \<sigma>) es2"])   
-  apply (simp add: iterm.rrename_comps) apply(subst irrename_itvsubst_comp) apply auto
-  apply(subst imkSubst_smap_irrename_inv) unfolding ssbij_def apply auto 
-  apply(subst irrename_eq_itvsubst_iVar'[of _ e1]) unfolding ssbij_def apply auto
-  apply(subst itvsubst_comp) 
-    subgoal by (metis SSupp_imkSubst imkSubst_smap_irrename_inv)
-    subgoal by (smt (verit, best) SSupp_def VVr_eq_Var card_of_subset_bound mem_Collect_eq not_in_supp_alt o_apply subsetI) 
-    subgoal apply(rule itvsubst_cong)
-      subgoal using SSupp_irrename_bound by blast
-      subgoal using card_SSupp_itvsubst_imkSubst_irrename_inv ssbij_def by auto
-   subgoal for x apply simp apply(subst iterm.subst(1))
-      subgoal using card_SSupp_imkSubst_irrename_inv[unfolded ssbij_def] by auto
-      subgoal by simp . . . .
-
-lemma hred_reneqv: 
-assumes "reneqv e ee" "hred e e'" "hred ee ee'" 
-shows "reneqv e' ee'"
-using assms reneqv_head_reduction unfolding hred_def by auto 
-
-lemma hred_reneqvS: 
-assumes "reneqvS es ees" "stream_all2 hred es es'" and "stream_all2 hred ees ees'"
-shows "reneqvS es' ees'"
-using hred_reneqv assms unfolding reneqvS_def stream_all2_iff_snth sset_range  
-by simp (smt (verit) image_iff)
-
-lemma hred_uniform: 
-assumes "hred e e'" and "uniform e"
-shows "uniform e'"
-using assms hred_reneqv unfolding uniform_def3 by blast
-
-lemma hred_uniformS: 
-assumes "stream_all2 hred es es'" and "uniformS es"
-shows "uniformS es'"
-using assms hred_reneqvS unfolding uniformS_def3 by blast
-
-
 
 
 (* TO DOCUMENT in the paper: 
@@ -455,45 +410,15 @@ unfolding Tmap_def ssbij_def wfBij_presSuper by auto
 
 
 (* Other properties: *)
-
 (* The following captures the freshness assumption for beta (coming from the "parameter" 
-predicate hred as part of ustepD. So fresh induction will use both 
-the avoidance from the ustepD Xi rule and this one (for hred).  Contrast this with 
+predicate hred as part of ustep. So fresh induction will use both 
+the avoidance from the ustep Xi rule and this one (for hred).  Contrast this with 
 beta, which does not "hide" any freshness assumptions inside parameter predicates, 
 so its rule induction covers both beta and Xi. *)
-lemma hred_eq_avoid: 
-assumes A: "small A" and r: "hred e e'"
-shows "\<exists> xs e1 es2. dsset xs \<inter> \<Union> (FFVars ` (sset es2)) = {} \<and> dsset xs \<inter> A = {} \<and>
-            e = iApp (iLam xs e1) es2 \<and> e' = itvsubst (imkSubst xs es2) e1"
-proof-
-  obtain xs e1 es2 where e: "e = iApp (iLam xs e1) es2" and e': "e' = itvsubst (imkSubst xs es2) e1" 
-  using r unfolding hred_def by auto
-  define B where B: "B = A \<union> \<Union> (FFVars ` (sset es2))"
-  have "small B" unfolding B by (metis A Tfvars.simps Un_absorb small_Un ssmall_Tfvars)
-  then obtain xs' e1' where 0: "iLam xs e1 = iLam xs' e1'" "dsset xs' \<inter> B = {}"
-  using iLam_avoid by (meson small_def)
 
-  obtain f where f: "bij f" "|supp f| <o |UNIV::ivar set|" "id_on (FFVars (iLam xs e1)) f" 
-  and 1: "xs' = dsmap f xs" "e1' = irrename f e1" using 0(1) unfolding iLam_inject by auto
-  show ?thesis apply(intro exI[of _ xs'] exI[of _ e1'] exI[of _ es2]) apply(intro conjI)
-    subgoal using 0(2) unfolding B by auto
-    subgoal using 0(2) unfolding B by auto
-    subgoal unfolding e 0(1) ..
-    subgoal unfolding e' 0(1) 1 apply(subst irrename_eq_itvsubst_iVar')
-      subgoal by fact  subgoal by fact
-      subgoal apply(subst itvsubst_comp)
-        subgoal by simp
-        subgoal by (simp add: f(2))   
-        apply(subst itvsubst_cong) apply auto 
-        apply (simp add: SSupp_itvsubst_bound f(2))
-        by (metis (full_types) "0"(1) "1"(1) Diff_iff f(1) f(3) id_on_def imkSubst_idle 
-          imkSubst_smap iterm.set(3)) . . 
-qed
+thm hred_eq_avoid
 
-lemma hred_FFVars: "hred e e' \<Longrightarrow> FFVars e' \<subseteq> FFVars e"
-unfolding hred_def by auto (metis imkSubst_def iterm.set(1) singletonD snth_sset)+
-
-lemma ustepD_FFVars: "ustepD es es' \<Longrightarrow> (\<forall>i. FFVars (snth es' i) \<subseteq> FFVars (snth es i))"
+lemma ustepD_FFVars: "ustepD d es es' \<Longrightarrow> (\<forall>i. FFVars (snth es' i) \<subseteq> FFVars (snth es i))"
 apply(induct rule: ustepD.induct) 
 using hred_FFVars apply (auto simp: sset_smap2 sset_range snth_sflat stream_all2_iff_snth )
 by (metis in_mono nat2_nat1 snth2.simps)
