thys/Untyped_Lambda_Calculus/LC_Head_Reduction.thy
@@ -1,0 +1,8 @@
+theory LC_Head_Reduction
+imports LC2
+begin
+
+definition red where 
+"red e ee \<equiv> \<exists>x e1 e2. e = App (Lam x e1) e2 \<and> ee = tvsubst (Var(x:=e2)) e1"
+
+end
